concurrent/promise_free/elimination_stack/StackIA.v
@@ -1,0 +1,206 @@
+Require Import CRIS.common.CRIS.
+From CRIS.scheduler Require Import SchHeader SchI SchA SchTactics.
+From CRIS.promise_free.algebra Require Import HistoryRA AtomicRA.
+From CRIS.promise_free.system
+  Require Import SystemHeader SystemA SystemTactics.
+From CRIS.promise_free.elimination_stack
+  Require Import StackHeader StackA StackI.
+From CRIS.promise_free.elimination_stack
+  Require Import StackIANewStack StackIAPush StackIAPop.
+From CRIS.helping Require Export HelpingTactics.
+
+Module StackIM. Section StackIM.
+  Context `{!crisG Γ Σ α β τ _S _I,
+    _HIST : !histGS, _ATOMIC : !atomicG, _SYS : !sysGS,
+    _STACK : !stackG, _HELP : !helpingGS, _SCH : !schGS}.
+
+  Context (mn : string) (sp_user sp : specmap).
+
+  Local Definition SysF := CFilter.filter (Helping.exports mn)
+    (SystemA.t sp_user (↑stackN) sp).
+  Local Definition SchF := CFilter.filter (Helping.exports mn) SchI.t.
+  Local Definition MA :=
+    ((StackM.t mn (SystemA.sp sp_user (↑stackN)) ★
+        HelpingOn.t mn StackM.jobCode) ★ SysF) ★ SchF.
+  Local Definition MI :=
+    ((CFilter.filter (Helping.exports mn) StackI.t ★
+        HelpingDummy.t mn) ★ SysF) ★ SchF.
+  Local Notation Ist :=
+    (IstProd (IstSB [mn] (IstHelp IstTrue ⊤)) IstEq).
+
+  Lemma sim (Hsys : (SystemA.sp sp_user (↑stackN)) ⊆ sp) :
+    ISim.t open MA MI (hinv_ownE ⊤) Ist.
+  Proof.
+    rewrite /MA /MI.
+    rewrite -(assoc Mod.add
+      (StackM.t mn (SystemA.sp sp_user (↑stackN)) ★
+        HelpingOn.t mn StackM.jobCode) SysF SchF).
+    rewrite -(assoc Mod.add
+      (CFilter.filter (Helping.exports mn) StackI.t ★
+        HelpingDummy.t mn) SysF SchF).
+    cStartModSim.
+    { rewrite !assoc. exact (new_stack_simF mn sp_user sp). }
+    { rewrite !assoc. exact (push_simF mn sp_user sp). }
+    { rewrite !assoc. exact (pop_simF mn sp_user sp). }
+    { cStartFunSim; cStepsT. cStepsT; ss. }
+    { cStartFunSim; cStepsT. cStepsT; ss. }
+    all: try mod_tac.
+    { iIntros "HE". rewrite /IstProd /IstSB /IstHelp /IstTrue /IstEq.
+      repeat iExists _; iFrame; iPureIntro; splits; eauto; ss. }
+  Qed.
+End StackIM. End StackIM.
+
+From CRIS.helping Require Export HelpingFacts.
+
+Module StackIA. Section StackIA.
+  Context `{!crisG Γ Σ α β τ _S _I,
+    _HIST : !histGS, _ATOMIC : !atomicG, _SYS : !sysGS,
+    _STACK : !stackG, _HELP : !helpingGS, _SCH : !schGS}.
+
+  Lemma ctxr (sp_user sp : specmap) :
+    (SystemA.sp sp_user (↑stackN)) ⊆ sp →
+    help_init_cond ⊢
+      ctx_refines
+        (StackI.t ★ SystemA.t sp_user (↑stackN) sp ★ SchI.t)
+        (StackA.t (SystemA.sp sp_user (↑stackN)) ★
+          SystemA.t sp_user (↑stackN) sp ★ SchI.t).
+  Proof.
+    intros Hsys.
+    iIntros "H".
+    iApply (helping_main
+      (fun mn => StackM.t mn (SystemA.sp sp_user (↑stackN)))
+      (StackA.t (SystemA.sp sp_user (↑stackN))) StackI.t
+      (SystemA.t sp_user (↑stackN) sp)
+      StackM.jobCode with "H").
+    { iIntros (mn) "HE". rewrite !CFilter.filter_app.
+      (* intermediate refinement with helping facilities *)
+      rewrite comm assoc (comm _ (HelpingDummy.t mn)).
+      iApply ctxr_trans. iSplitL "HE".
+      { rewrite !assoc.
+        iApply (main_adequacy _ _ (hinv_ownE ⊤)
+          (IstProd (IstSB [mn] (IstHelp IstTrue ⊤)) IstEq)
+          (StackIM.sim mn sp_user sp Hsys)).
+        iExact "HE".
+      }
+      rewrite -!assoc. iApply ctxr_trans. iSplitR.
+      { ctxr_rotate. ctxr_swap. do 2 ctxr_rotate. ctxr_swap.
+        ctxr_rotate. ctxr_swap. do 3 ctxr_rotate. ctxr_refl. }
+      rewrite (comm Mod.add
+        (HelpingOn.t mn StackM.jobCode)
+        (CFilter.filter (Helping.exports mn) SchI.t)).
+      rewrite (assoc Mod.add
+        (CFilter.filter (Helping.exports mn)
+          (SystemA.t sp_user (↑stackN) sp))
+        (StackM.t mn (SystemA.sp sp_user (↑stackN)))
+        (CFilter.filter (Helping.exports mn) SchI.t ★
+          HelpingOn.t mn StackM.jobCode)).
+      rewrite (comm Mod.add
+        (CFilter.filter (Helping.exports mn)
+          (SystemA.t sp_user (↑stackN) sp))
+        (StackM.t mn (SystemA.sp sp_user (↑stackN)))).
+      rewrite -(assoc Mod.add
+        (StackM.t mn (SystemA.sp sp_user (↑stackN)))
+        (CFilter.filter (Helping.exports mn)
+          (SystemA.t sp_user (↑stackN) sp))
+        (CFilter.filter (Helping.exports mn) SchI.t ★
+          HelpingOn.t mn StackM.jobCode)).
+      ctxr_refl.
+    }
+
+    iIntros (mn). rewrite !CFilter.filter_app.
+    iApply ctxr_trans. iSplitR.
+    { do 3 ctxr_rotate. ctxr_swap. ctxr_refl. }
+
+    rewrite
+      (assoc _
+        (StackM.t mn (SystemA.sp sp_user (↑stackN)))).
+
+    iApply (main_adequacy _ _ emp%I
+      (IstProd
+        (IstSB
+          (Mod.scopes (StackA.t (SystemA.sp sp_user (↑stackN))) ++ [mn])
+          IstTrue)
+        IstEq)).
+    cStartModSim.
+    { (* new_stack *)
+      cStartFunSim.
+      rewrite /StackM.new_stack /StackA.new_stack /stack_atomic_fun.
+      cStepsS. cStepsT.
+      destruct _q as [[tid stid] V].
+      iDestruct "ASM" as "[-> TV]".
+      cForceT (tid, stid, V).
+      cForceT (tt↑). cForcesT.
+      iFrame "TV". repeat iSplit; eauto.
+      iApply wsim_bind. iSplitL "IST".
+      { iApply isim_wsim. iIntros "WINV". iApply isim_refl.
+        - intros; ss.
+        - intros; ss.
+        - iFrame. }
+      iIntros (????) "[-> IST]".
+      sYields. sYieldS.
+      iDestruct "GRT" as "[%EQ GRT]".
+      subst _q0.
+      cForceS (_q↑, tt).
+      cForcesS. iFrame "GRT".
+      cStep. iFrame. auto.
+    }
+    { (* push *)
+      cStartFunSim.
+      rewrite /StackM.push /StackA.push /stack_atomic_fun.
+      cStepsS. cStepsT.
+      destruct _q as [[[[value γs] tid] stid] V].
+      iDestruct "ASM" as (stack) "[-> [#HANDLE TV]]".
+      cForceT (value, γs, tid, stid, V).
+      cForceT ((stack, value, γs)↑). cForcesT.
+      iFrame "HANDLE TV". repeat iSplit; eauto.
+      cStepsT.
+      cNormS.
+      iApply wsim_bind. iSplitL "IST".
+      { iApply isim_wsim. iIntros "WINV". iApply isim_refl.
+        - intros; ss.
+        - intros; ss.
+        - iFrame. }
+      iIntros (????) "[-> IST]".
+      cStepsT.
+      cInlineT. cStepsT. rewrite /HelpingOff.run. cStepsT.
+      aUnfoldS. aUnfoldT. sYields. sYieldS. cStepsS.
+      rewrite /StackM.jobCode. cForcesT; iFrame.
+      cStepsT. cForceS (inr _). cForcesS; iFrame.
+      sYields. sYieldS. cStepsS.
+      instantiate (1 := Val.zero↑).
+      iDestruct "GRT" as "[-> GRT]".
+      cForcesS. iFrame "GRT".
+      cStep. iFrame. auto.
+    }
+    { (* pop *)
+      cStartFunSim.
+      rewrite /StackM.pop /StackA.pop /stack_atomic_fun.
+      cStepsS. cStepsT.
+      destruct _q as [[[γs tid] stid] V].
+      cStepsS.
+      iDestruct "ASM" as "[%stack [-> [#HANDLE TV]]]".
+      cForceT (γs, tid, stid, V). cForcesT.
+      iSplitL "TV".
+      { iExists stack. iFrame "HANDLE TV". eauto. }
+      aAddY. sYields. case_match.
+      { cStepsT. cInlineT. cStepsT. rewrite /HelpingOff.help. cStepsT.
+        sYields. sYieldS.
+        aStep. iExists 0. iAuIntro.
+        iAaccIntro "% $ !>" with "". iSplit; first eauto.
+        iIntros "%ret_t $ !>"; iExists ret_t; iModIntro.
+        clear_st; iIntros (st_src st_tgt) "IST".
+        cStepsT. sYieldS. cForcesS; iFrame "GRT".
+        cStep. iFrame. auto.
+      }
+      cStepsT. sYieldS. aStep.
+      iExists 0. iAuIntro.
+      iAaccIntro "% $ !>" with "". iSplit; first eauto.
+      iIntros "%ret_t $ !>"; iExists ret_t; iModIntro.
+      clear_st; iIntros (st_src st_tgt) "IST".
+      cStepsT. sYieldS. cForcesS; iFrame "GRT".
+      cStep. iFrame. auto.
+    }
+    { iIntros "_"; repeat iExists _; repeat iSplit; eauto. }
+    iEmpIntro.
+  Qed.
+End StackIA. End StackIA.
