concurrent/promise_free/elimination_stack/StackIAPush.v
@@ -1,0 +1,1087 @@
+Require Import CRIS.common.CRIS.
+From CRIS.scheduler Require Import SchHeader SchI SchA SchTactics.
+From CRIS.promise_free.algebra Require Import HistoryRA AtomicRA.
+From CRIS.promise_free.system Require Import SystemHeader SystemA SystemTactics.
+From CRIS.promise_free.elimination_stack Require Import StackHeader StackA StackI.
+From CRIS.helping Require Import HelpingTactics HelpingFacts.
+
+Section StackIM.
+  Context `{!crisG Γ Σ α β τ _S _I, _HIST: !histGS, _ATOMIC: !atomicG,
+    _SYS: !sysGS, _STACK: !stackG, _HELP: !helpingGS, !schGS}.
+  Local Existing Instance stack_token_inG.
+  Context (mn : string) (sp_user sp : specmap).
+  Context (Hsys : (SystemA.sp sp_user (↑stackN)) ⊆ sp).
+
+  Local Definition SysF := CFilter.filter (Helping.exports mn)
+    (SystemA.t sp_user (↑stackN) sp).
+  Local Definition SchF := CFilter.filter (Helping.exports mn) SchI.t.
+  Local Definition MA :=
+    ((StackM.t mn (SystemA.sp sp_user (↑stackN)) ★
+        HelpingOn.t mn StackM.jobCode) ★ SysF) ★ SchF.
+  Local Definition MI :=
+    ((CFilter.filter (Helping.exports mn) StackI.t ★
+        HelpingDummy.t mn) ★ SysF) ★ SchF.
+  Local Notation Ist :=
+    (IstProd (IstSB [mn] (IstHelp IstTrue ⊤)) IstEq).
+
+  Local Lemma push_postcond_irrel value γs tid stid V V' :
+    postcond StackM.push_spec (value, γs, tid, stid, V) =
+    postcond StackM.push_spec (value, γs, tid, stid, V').
+  Proof. reflexivity. Qed.
+
+  Local Lemma cell_add_lt ζ from to msg ζ'
+      (ADD : Cell.add ζ from to msg ζ') :
+    Time.lt from to.
+  Proof. inversion ADD; done. Qed.
+
+  Lemma push_simF :
+    ISim.sim_fun open MA MI Ist (fid StackHdr.push).
+  Proof.
+    cStartFunSim. rewrite /StackI.push /StackM.push. cStepsS. cStepsT.
+    destruct _q as [[[[value γs] tid] stid] V].
+    iDestruct "ASM" as (stack) "[[-> ->] [#HANDLE TV]]".
+    cStepsS. cStepsT.
+    cStepsT.
+    iApply wsim_system_yield_ir; ss.
+    { apply bool_decide_true. split; last done.
+      rewrite /Helping.exports elem_of_union !elem_of_singleton.
+      intros [EQ|EQ]; unfold Helping.run, Helping.help in EQ; discriminate. }
+    iFrame "TV IST".
+    clear dependent st_src st_tgt.
+    iIntros (st_src st_tgt) "IST TV".
+    iApply wsim_system_yield_src. cStepsS.
+    iApply wsim_helping_run; [simpl_map; s; f_equal|].
+    iIntros (reqid) "HELP".
+    rewrite SRed.bind SBRed.bind bind_bind. cNormT.
+    iApply wsim_reset.
+    cCoind CIH g' __ with st_src st_tgt V.
+    iIntros "[#HANDLE [IST [TV HELP]]] /=".
+    rewrite StackI.push_loop_unfold /StackI.push_once.
+    cStepsS. cStepsT. cHideS. cHideT. sYields.
+    rewrite /stack_handle.
+    iDestruct "HANDLE" as
+      (stack_loc γstackinv γh γslot ζh_seen ζo_seen γguard ζguard γnm)
+      "[%STACK [#Hinv [#SNh [#SNo #SNg]]]]".
+    destruct STACK as [-> STACK_BASE].
+    sYield. cStepsT.
+    iEval (rewrite IstHelp_nested_equiv) in "IST".
+    iInv "Hinv" with "[IST]" as "[IST INV]" "ACC";
+      first by iFrame.
+    iEval (rewrite stack_inv'_eq; solve_base_sl_red) in "INV".
+    iDestruct "INV" as
+      (vs head offer ζh ζo Vbh Vbo Vh Vo targets nodes)
+      "[Hs [HEAD [HPURE [CHAIN [SLOT [OPURE [OFFER [TARGETS REG]]]]]]]]".
+    iEval (rewrite syn_AtomicPtsTo_red AtomicPtsTo_eq /AtomicPtsTo_def) in "HEAD".
+    iDestruct "HEAD" as (txh) "HEAD".
+    cInlineT.
+    cForceT (meta1 (tid, stid, stack_loc, Ordering.acqrel,
+      ζh, ζh_seen, txh, γh, 1%Qp, CASOnly, V, Vbh))%cris.
+    cForcesT. iFrame "TV SNh HEAD". iSplit; eauto.
+    iSplit; ss.
+    rewrite shift_0. ss.
+    cStepT.
+    cStepT.
+    cStepT.
+    iDestruct "GRT" as
+      "[-> [%ζread [%fread [%na [%vret [%vactual [%Vmsg [%V1 [HREAD [#SNh1 [HEAD TV]]]]]]]]]]]".
+    iDestruct "HREAD" as
+      %[-> [Hval [Hseen [Hle [Hget [HVle HVmsg]]]]]].
+    iPoseProof "HPURE" as "#HPUREcopy".
+    iDestruct "HPUREcopy" as
+      %(CURh & CASHh & PTRh & HEADH & LINKS & SENTh).
+    pose proof (Hle _ _ _ Hget) as Hgeth.
+    destruct (PTRh _ _ _ _ _ Hgeth) as
+      (head_loc & Vguard & Hactual & Htarget & Hsafe).
+    subst vactual.
+    pose proof (StackHdr.le_vptr_eq Hval) as Hret. subst vret.
+    simpl in HVmsg.
+    iAssert (⌜current_message ζh head Vh ∧ cas_history ζh ∧
+      pointer_history (stack_loc >> 2) targets ζh ∧
+      head_history (stack_loc >> 2) nodes ζh ∧
+      node_links (stack_loc >> 2) targets nodes ∧
+      (∃ Vsent, (stack_loc >> 2, Vsent) ∈ targets)⌝)%I
+      as "HPURE"; first done.
+    iMod ("ACC" with "[//]") as "[ACC _]".
+    iMod ("ACC" with
+      "[Hs HEAD HPURE CHAIN SLOT OPURE OFFER TARGETS REG] IST") as "IST".
+    { iEval (rewrite stack_inv'_eq; solve_base_sl_red).
+      iExists vs, head, offer, ζh, ζo, Vbh, Vbo, Vh, Vo, targets, nodes.
+      solve_base_sl_red; iFrame "Hs HPURE CHAIN SLOT OPURE OFFER TARGETS REG".
+      rewrite syn_AtomicPtsTo_red AtomicPtsTo_eq /AtomicPtsTo_def.
+      iExists txh. iFrame. }
+    iEval (rewrite -IstHelp_nested_equiv) in "IST".
+    cStepsT.
+    sYield. cStepsT. cInlineT.
+    cForceT (tid, stid, 3, V1). cForcesT. iFrame. iSplit; eauto.
+    cStepsT.
+    iDestruct "GRT" as
+      "[-> [%node [%V2 [[-> %HV12] [TV [FA NODE]]]]]]".
+    iEval (rewrite hist_freeable_eq /hist_freeable_def) in "FA".
+    iDestruct "FA" as (alloc_tid alloc_bid) "[%NODEBASE _]".
+    assert (Loc.ofs node = 0%Z) as NODE_BASE by (rewrite NODEBASE; done).
+    rewrite 2!own_loc_na_vec_cons own_loc_na_vec_singleton.
+    cStepsT.
+    iDestruct "NODE" as "[NODE0 [NODE1 NODE2]]".
+    iEval (rewrite shift_nat_assoc /=) in "NODE2".
+    sYields. cStepsT. cInlineT.
+    cForceT (meta0 (tid, stid, node, Val.zero, Ordering.na, V2))%cris.
+    cForcesT. rewrite shift_0. iFrame "TV". iSplitL "NODE0".
+    { do 2 (iSplit; eauto). iApply own_loc_na_own_loc; done. }
+    cStepsT.
+    iDestruct "GRT" as "[-> [%V3 [[-> %HV23] [NODE0 TV]]]]".
+    iPoseProof (view_at_cur_mon_pred V2 V3 HV23 with "NODE1") as "NODE1".
+    iPoseProof (view_at_cur_mon_pred V2 V3 HV23 with "NODE2") as "NODE2".
+    cStepsT.
+    sYields. cStepsT. cInlineT.
+    cForceT (meta0
+      (tid, stid, node >> 1, Val.Vptr head_loc, Ordering.na, V3))%cris.
+    cForcesT. iFrame "TV". iSplitL "NODE1".
+    { do 2 (iSplit; eauto). iApply own_loc_na_own_loc; done. }
+    cStepsT.
+    iDestruct "GRT" as "[-> [%V4 [[-> %HV34] [NODE1 TV]]]]".
+    iPoseProof (view_at_cur_mon_pred V3 V4 HV34 with "NODE0") as "NODE0".
+    iPoseProof (view_at_cur_mon_pred V3 V4 HV34 with "NODE2") as "NODE2".
+    cStepsT.
+    sYields. cStepsT. cInlineT.
+    cForceT (meta0
+      (tid, stid, node >> 2, StackHdr.encode value, Ordering.na, V4))%cris.
+    cForcesT. iFrame "TV". iSplitL "NODE2".
+    { do 2 (iSplit; eauto). iApply own_loc_na_own_loc; done. }
+    cStepsT.
+    iDestruct "GRT" as "[-> [%V5 [[-> %HV45] [NODE2 TV]]]]".
+    iPoseProof (view_at_cur_mon_pred V4 V5 HV45 with "NODE0") as "NODE0".
+    iPoseProof (view_at_cur_mon_pred V4 V5 HV45 with "NODE1") as "NODE1".
+    cStepsT.
+    sYields. cStepsT. cInlineT.
+    inversion HV12 as [Hrel12 Hcur12 Hacq12].
+    inversion HV23 as [Hrel23 Hcur23 Hacq23].
+    inversion HV34 as [Hrel34 Hcur34 Hacq34].
+    inversion HV45 as [Hrel45 Hcur45 Hacq45].
+    assert (Hcur15 : View.le (TView.cur V1) (TView.cur V5)) by
+      (etrans; [exact Hcur12|]; etrans; [exact Hcur23|];
+       etrans; [exact Hcur34|exact Hcur45]).
+    assert (HcurV5 : View.le (TView.cur V) (TView.cur V5)) by
+      (etrans; [exact HVle|exact Hcur15]).
+    iPoseProof (view_at_view_mon_pred
+      (view_at (AtomicSeen stack_loc γh ζread)) _ _ Hcur15
+      with "SNh1") as "#SNh5".
+    iPoseProof (view_at_view_mon_pred
+      (view_at (AtomicSeen (stack_loc >> 2) γguard ζguard)) _ _ HcurV5
+      with "SNg") as "#SNg5".
+    iEval (rewrite IstHelp_nested_equiv) in "IST".
+    iInv "Hinv" with "[IST]" as "[IST INV]" "ACC";
+      first by iFrame.
+    iEval (rewrite stack_inv'_eq; solve_base_sl_red) in "INV".
+    iDestruct "INV" as
+      (vsc headc offerc ζhc ζoc Vbhc Vboc Vhc Voc targetsc nodesc)
+      "[Hsc [HEADc [HPUREc [CHAINc [SLOTc [OPUREc [OFFERc [TARGETSc REGc]]]]]]]]".
+    iEval (rewrite syn_AtomicPtsTo_red AtomicPtsTo_eq /AtomicPtsTo_def)
+      in "HEADc".
+    iDestruct "HEADc" as (txhc) "HEADc".
+    iPoseProof (AtomicPtsToX_AtomicSeen_latest with "HEADc SNh5")
+      as "%Hread_cur".
+    pose proof (Hread_cur _ _ _ Hget) as Hget_cur.
+    iPoseProof "HPUREc" as "#HPUREcopyc".
+    iDestruct "HPUREcopyc" as
+      %(CURhc & CASHhc & PTRhc & HEADHc & LINKSc & SENTc).
+    destruct (PTRhc _ _ _ _ _ Hget_cur) as
+      (Vhead & Vguardc & Hheadeq & Htargetc & Hsafec).
+    inversion Hheadeq; subst Vhead.
+    iDestruct (node_registry_fresh γnm with "NODE1 REGc") as
+      "[%FRESH [NODE1 REGc]]".
+    iMod (AtomicPtsTo_from_na node Val.zero with "NODE0") as
+      "[%γnodeguard [%tg [%fg [%LTg [%Vg [%nag [%Vg_le [SWg PTg]]]]]]]]".
+    iMod (AtomicPtsTo_from_na (node >> 1) (Val.Vptr head_loc)
+      with "NODE1") as
+      "[%γnext [%tn [%fn [%LTn [%Vn [%nan [%Vn_le [SWn PTn]]]]]]]]".
+    set (dnew := NodeDesc head_loc value (TView.cur V5)).
+    iAssert (target_record (node, TView.cur V5))%I
+      with "[PTg SWg]" as "NEW_TARGET".
+    { iExists fg, tg, LTg, Vg, nag, γnodeguard. iFrame. }
+    iAssert (node_record node dnew)%I with "[PTn SWn]" as "NEW_NODE".
+    { rewrite /node_record /immutable_field /dnew /=.
+      iExists fn, tn, LTn, Vn, (TView.cur V5), nan, γnext.
+      iFrame. iPureIntro. split; first done. exact Vn_le. }
+    iAssert (live_value node dnew)%I with "[NODE2]" as "NEW_VALUE".
+    { rewrite /live_value /dnew /=. iExists (TView.cur V5). iFrame. done. }
+    assert (NODE_NE : node ≠ stack_loc >> 2) by
+      (eapply base_loc_not_sentinel; eauto).
+    cForceT (tid, stid, stack_loc, Val.Vptr head_loc, Val.Vptr node,
+      Ordering.relaxed, Ordering.acqrel, V5, γh, ζread, Vbhc, txhc,
+      ζhc, CASOnly, target_pool targetsc)%cris.
+    cForcesT. rewrite shift_0.
+    iFrame "TV SNh5 HEADc TARGETSc".
+    change (View.le Vmsg (TView.cur V1)) in HVmsg.
+    iSplit; eauto.
+    { iSplitL ""; first done.
+      iSplitL "".
+      { iPureIntro. repeat split; eauto.
+        intros t f v0 V0 b Htime Hget0.
+        destruct (PTRhc _ _ _ _ _ Hget0) as
+          (loc0 & Vguard0 & EQ & IN & SAFE).
+        rewrite EQ. done. }
+      iModIntro. iIntros "POOL". iModIntro.
+      iSplit.
+      { destruct Hsafec as [HSENT|Hguard].
+        - subst head_loc.
+          iDestruct (target_pool_lookup targetsc
+            (stack_loc >> 2, Vguardc) Htargetc with "POOL") as "REC".
+          iDestruct (target_record_prim with "REC") as
+            (q C Vp) "PR".
+          iExists q, C, Vp, γguard, ζguard. iFrame "PR SNg5".
+        - assert (Hguard5 : View.le Vguardc (TView.cur V5)) by
+            (etrans; [exact Hguard|]; etrans; [exact HVmsg|exact Hcur15]).
+          iDestruct (target_pool_lookup targetsc
+            (head_loc, Vguardc) Htargetc with "POOL") as "REC".
+          iDestruct (target_record_take (head_loc, Vguardc)
+            (TView.cur V5) Hguard5 with "REC") as
+            (q C Vp γp Cp) "[PR #SEEN]".
+          iExists q, C, Vp, γp, Cp. iFrame "PR SEEN". }
+      iIntros (t f l' V' b) "%OTHER".
+      destruct OTHER as (Htime & Hget' & Hne).
+      destruct (PTRhc _ _ _ _ _ Hget') as
+        (loc' & Vguard' & EQ & IN & SAFE).
+      inversion EQ; subst loc'.
+      iDestruct (target_pool_lookup targetsc (l', Vguard') IN
+        with "POOL") as "REC".
+      iDestruct (target_record_prim with "REC") as (q C Vp) "PR".
+      iExists q, C, Vp. done. }
+    cStepT. cStepT. cStepT.
+    iDestruct "GRT" as "[%EQ GRT]". subst _q0.
+    iDestruct "GRT" as
+      (ret ζafter ζnew tcas fcas LTcas vseen Vread bcas V6)
+      "[%PURE [TV [#SNh6 [TARGETSc RESULT]]]]".
+    destruct PURE as
+      (QRET & Hread_after & Hafter_new & Hgetcas & Htimecas & HV56).
+    iAssert (⌜current_message ζhc headc Vhc ∧ cas_history ζhc ∧
+      pointer_history (stack_loc >> 2) targetsc ζhc ∧
+      head_history (stack_loc >> 2) nodesc ζhc ∧
+      node_links (stack_loc >> 2) targetsc nodesc ∧
+      (∃ Vsent, (stack_loc >> 2, Vsent) ∈ targetsc)⌝)%I
+      as "#HPUREc"; first done.
+    iDestruct "RESULT" as "[FAIL|SUCCESS]".
+    - iDestruct "FAIL" as "[%FAIL HEADc]".
+      destruct FAIL as (-> & Hneq & HVread & Hsame). subst ζnew.
+      subst _q.
+      iMod ("ACC" with "[//]") as "[ACC _]".
+      iMod ("ACC" with
+        "[Hsc HEADc HPUREc CHAINc SLOTc OPUREc OFFERc TARGETSc REGc] IST")
+        as "IST".
+      { iEval (rewrite stack_inv'_eq; solve_base_sl_red).
+        iExists vsc, headc, offerc, ζhc, ζoc, Vbhc, Vboc, Vhc, Voc,
+          targetsc, nodesc.
+        solve_base_sl_red.
+        iFrame "Hsc CHAINc SLOTc OFFERc TARGETSc REGc".
+        iFrame "HPUREc OPUREc".
+        rewrite syn_AtomicPtsTo_red AtomicPtsTo_eq /AtomicPtsTo_def.
+        iExists txhc. iFrame. }
+      iEval (rewrite -IstHelp_nested_equiv) in "IST".
+      cStepsT. sYields. cStepsT.
+      cInlineT.
+      cForceT (tid, stid, 3, V6). cForcesT. iFrame. iSplit; eauto.
+      cStepsT.
+      iDestruct "GRT" as
+        "[-> [%offer_loc [%V7 [[-> %HV67] [TV [FA OFFER]]]]]]".
+      iEval (rewrite hist_freeable_eq /hist_freeable_def) in "FA".
+      iDestruct "FA" as (offer_tid offer_bid) "[%OFFERBASE _]".
+      assert (Loc.ofs offer_loc = 0%Z) as OFFER_BASE by
+        (rewrite OFFERBASE; done).
+      rewrite 2!own_loc_na_vec_cons own_loc_na_vec_singleton.
+      cStepsT. iDestruct "OFFER" as "[OFFER0 [OFFER1 OFFER2]]".
+      iEval (rewrite shift_nat_assoc /=) in "OFFER2".
+      sYields. cStepsT. cInlineT.
+      cForceT (meta0
+        (tid, stid, offer_loc, Val.zero, Ordering.na, V7))%cris.
+      cForcesT. rewrite shift_0. iFrame "TV". iSplitL "OFFER0".
+      { do 2 (iSplit; eauto). iApply own_loc_na_own_loc; done. }
+      cStepsT.
+      iDestruct "GRT" as "[-> [%V8 [[-> %HV78] [OFFER0 TV]]]]".
+      iPoseProof (view_at_cur_mon_pred V7 V8 HV78 with "OFFER1")
+        as "OFFER1".
+      iPoseProof (view_at_cur_mon_pred V7 V8 HV78 with "OFFER2")
+        as "OFFER2".
+      cStepsT. sYields. cStepsT. cInlineT.
+      cForceT (meta0
+        (tid, stid, offer_loc >> 1, Val.zero, Ordering.na, V8))%cris.
+      cForcesT. iFrame "TV". iSplitL "OFFER1".
+      { do 2 (iSplit; eauto). iApply own_loc_na_own_loc; done. }
+      cStepsT.
+      iDestruct "GRT" as "[-> [%V9 [[-> %HV89] [OFFER1 TV]]]]".
+      iPoseProof (view_at_cur_mon_pred V8 V9 HV89 with "OFFER0")
+        as "OFFER0".
+      iPoseProof (view_at_cur_mon_pred V8 V9 HV89 with "OFFER2")
+        as "OFFER2".
+      cStepsT. sYields. cStepsT. cInlineT.
+      cForceT (meta0 (tid, stid, offer_loc >> 2,
+        StackHdr.encode value, Ordering.na, V9))%cris.
+      cForcesT. iFrame "TV". iSplitL "OFFER2".
+      { do 2 (iSplit; eauto). iApply own_loc_na_own_loc; done. }
+      cStepsT.
+      iDestruct "GRT" as "[-> [%V10 [[-> %HV910] [OFFER2 TV]]]]".
+      iPoseProof (view_at_cur_mon_pred V9 V10 HV910 with "OFFER0")
+        as "OFFER0".
+      iPoseProof (view_at_cur_mon_pred V9 V10 HV910 with "OFFER1")
+        as "OFFER1".
+      cStepsT.
+      inversion HV56 as [Hrel56 Hcur56 Hacq56].
+      inversion HV67 as [Hrel67 Hcur67 Hacq67].
+      inversion HV78 as [Hrel78 Hcur78 Hacq78].
+      inversion HV89 as [Hrel89 Hcur89 Hacq89].
+      inversion HV910 as [Hrel910 Hcur910 Hacq910].
+      assert (HcurV10 : View.le (TView.cur V) (TView.cur V10)) by
+        (etrans; [exact HcurV5|]; etrans; [exact Hcur56|];
+         etrans; [exact Hcur67|]; etrans; [exact Hcur78|];
+         etrans; [exact Hcur89|exact Hcur910]).
+      iPoseProof (view_at_view_mon_pred
+        (view_at (AtomicSeen (stack_loc >> 1) γslot ζo_seen)) _ _ HcurV10
+        with "SNo") as "#SNo10".
+      iPoseProof (view_at_view_mon_pred
+        (view_at (AtomicSeen (stack_loc >> 2) γguard ζguard)) _ _ HcurV10
+        with "SNg") as "#SNg10".
+      iMod (AtomicPtsTo_from_na offer_loc Val.zero with "OFFER0") as
+        "[%γoffer_guard [%tog [%fog [%LTog [%Vog [%naog [%Vog_le [SWog PTog]]]]]]]]".
+      iMod (AtomicPtsTo_from_na (offer_loc >> 1) Val.zero
+        with "OFFER1") as
+        "[%γstate [%tos [%fos [%LTos [%Vos [%naos [%Vos_le [SWos STATE]]]]]]]]".
+      iPoseProof (AtomicSWriter_AtomicSeen with "SWog") as "#SNoffer10".
+      iAssert (target_record (offer_loc, TView.cur V10))%I
+        with "[PTog SWog]" as "OFFER_TARGET".
+      { iExists fog, tog, LTog, Vog, naog, γoffer_guard. iFrame. }
+      iPoseProof (AtomicSWriter_AtomicSeen with "SWos") as "#SNstate".
+      iPoseProof (atomic_pts_to_swriter_to_cas with "STATE SWos")
+        as "STATE".
+      sYields. cStepsT.
+      iEval (rewrite IstHelp_nested_equiv) in "IST".
+      iInv "Hinv" with "[IST]" as "[IST INV]" "ACC";
+        first by iFrame.
+      iEval (rewrite stack_inv'_eq; solve_base_sl_red) in "INV".
+      iDestruct "INV" as
+        (vsd headd offerd ζhd ζod Vbhd Vbod Vhd Vod targetsd nodesd)
+        "[Hsd [HEADd [HPUREd [CHAINd [SLOTd [OPUREd [OFFERd [TARGETSd REGd]]]]]]]]".
+      iEval (rewrite syn_AtomicPtsTo_red AtomicPtsTo_eq /AtomicPtsTo_def)
+        in "SLOTd".
+      iDestruct "SLOTd" as (txod) "SLOTd".
+      iPoseProof (AtomicPtsToX_AtomicSeen_latest with "SLOTd SNo10")
+        as "%Hslot_seen".
+      iDestruct "HPUREd" as
+        %(CURhd & CASHhd & PTRhd & HEADHd & LINKSd & SENTd).
+      iDestruct "OPUREd" as %(CURod & CASHod & PTRod).
+      cInlineT.
+      cForceT (tid, stid, stack_loc >> 1, Val.Vptr (stack_loc >> 2),
+        Val.Vptr offer_loc, Ordering.relaxed, Ordering.acqrel, V10,
+        γslot, ζo_seen, Vbod, txod, ζod, CASOnly,
+        target_pool ((offer_loc, TView.cur V10) :: targetsd))%cris.
+      cForcesT. iFrame "TV SNo10 SLOTd".
+      iFrame "OFFER_TARGET TARGETSd".
+      iSplit; eauto.
+      { iSplitL ""; first done.
+        iSplitL "".
+        { iPureIntro. repeat split; eauto.
+          intros t f v0 V0 b Htime Hget0.
+          destruct (PTRod _ _ _ _ _ Hget0) as
+            (loc0 & Vguard0 & EQ & IN & SAFE).
+          rewrite EQ. done. }
+        iModIntro. iIntros "POOL". iModIntro.
+        iSplit.
+        { destruct SENTd as (Vsent & INsent).
+          iDestruct (target_pool_lookup
+            ((offer_loc, TView.cur V10) :: targetsd)
+            (stack_loc >> 2, Vsent) with "POOL") as "REC".
+          { right; exact INsent. }
+          iDestruct (target_record_prim with "REC") as (q C Vp) "PR".
+          iExists q, C, Vp, γguard, ζguard. iFrame "PR SNg10". }
+        iIntros (t f l' V' b) "%OTHER".
+        destruct OTHER as (Htime & Hget' & Hne).
+        destruct (PTRod _ _ _ _ _ Hget') as
+          (loc' & Vguard' & EQ & IN & SAFE).
+        inversion EQ; subst loc'.
+        iDestruct (target_pool_lookup
+          ((offer_loc, TView.cur V10) :: targetsd)
+          (l', Vguard') with "POOL") as "REC".
+        { right; exact IN. }
+        iDestruct (target_record_prim with "REC") as (q C Vp) "PR".
+        iExists q, C, Vp. done. }
+      cStepT. cStepT. cStepT.
+      iDestruct "GRT" as "[%EQP GRT]". subst _q0.
+      iDestruct "GRT" as
+        (published ζpubread ζpubnew tpub fpub LTpub vpub Vpubread bpub V11)
+        "[%PUBPURE [TV [#SNo11 [[OFFER_TARGET TARGETSd] PUBRESULT]]]]".
+      destruct PUBPURE as
+        (QPUB & Hseen_pub & Hpubread_new & Hgetpub & Htimepub & HV1011).
+      inversion HV1011 as [Hrel1011 Hcur1011 Hacq1011].
+      iAssert (⌜current_message ζhd headd Vhd ∧ cas_history ζhd ∧
+        pointer_history (stack_loc >> 2) targetsd ζhd ∧
+        head_history (stack_loc >> 2) nodesd ζhd ∧
+        node_links (stack_loc >> 2) targetsd nodesd ∧
+        (∃ Vsent, (stack_loc >> 2, Vsent) ∈ targetsd)⌝)%I
+        as "#HPUREd"; first done.
+      iAssert (⌜current_message ζod offerd Vod ∧ cas_history ζod ∧
+        pointer_history (stack_loc >> 2) targetsd ζod⌝)%I
+        as "#OPUREd"; first done.
+      iDestruct "PUBRESULT" as "[PUBFAIL|PUBSUCCESS]".
+      { iDestruct "PUBFAIL" as "[%PUBFAIL SLOTd]".
+        destruct PUBFAIL as (-> & Hpubneq & HVpubread & Hpubsame).
+        subst ζpubnew. subst _q.
+        iMod ("ACC" with "[//]") as "[ACC _]".
+        iMod ("ACC" with
+          "[Hsd HEADd HPUREd CHAINd SLOTd OPUREd OFFERd TARGETSd REGd] IST")
+          as "IST".
+        { iEval (rewrite stack_inv'_eq; solve_base_sl_red).
+          iExists vsd, headd, offerd, ζhd, ζod, Vbhd, Vbod, Vhd, Vod,
+            targetsd, nodesd.
+          solve_base_sl_red.
+          iFrame "Hsd HEADd HPUREd CHAINd OPUREd OFFERd TARGETSd REGd".
+          rewrite syn_AtomicPtsTo_red AtomicPtsTo_eq /AtomicPtsTo_def.
+          iExists txod. iFrame. }
+        iEval (rewrite -IstHelp_nested_equiv) in "IST".
+        cStepsT. sYields. cStepsT.
+        assert (HcurV11 : View.le (TView.cur V) (TView.cur V11)) by
+          (etrans; [exact HcurV10|exact Hcur1011]).
+        iPoseProof (view_at_view_mon_pred
+          (view_at (AtomicSeen stack_loc γh ζh_seen)) _ _ HcurV11
+          with "SNh") as "#SNh11".
+        iPoseProof (view_at_view_mon_pred
+          (view_at (AtomicSeen (stack_loc >> 2) γguard ζguard)) _ _ HcurV11
+          with "SNg") as "#SNg11".
+        iAssert (stack_handle γs (Val.Vptr stack_loc) (TView.cur V11))%I
+          with "[Hinv]" as "#HANDLE11".
+        { iExists stack_loc, γstackinv, γh, γslot, ζh_seen, ζpubread,
+            γguard, ζguard, γnm.
+          iSplit; first (iPureIntro; split; done).
+          iFrame "Hinv SNh11 SNo11 SNg11". }
+        unfold CS__.
+        unfold cris_s.
+        rewrite (push_postcond_irrel value γs tid stid V V11).
+        cNormS.
+        unfold CT__, cris_t. cNormT.
+        cByCoind CIH. iFrame "HANDLE11 TV IST HELP WINV". }
+      { iDestruct "PUBSUCCESS" as (Vpubwrite)
+          "[%PUBSUCCESS [_ SLOTd]]".
+        destruct PUBSUCCESS as
+          (-> & Heqpub & tpubwrite & HPUBADD & Hpubvrw & Hpubvrne &
+            Hpubnotle & HpubneV & Hpubord).
+        subst vpub.
+        subst _q.
+        assert (Htpubwrite : Time.lt tpub tpubwrite) by
+          (eapply cell_add_lt; exact HPUBADD).
+        assert (Htpub_ne : tpub ≠ tpubwrite) by
+          (intros ->; eapply Time.lt_strorder; exact Htpubwrite).
+        assert (Hgetpub_base :
+          Cell.get tpub ζod =
+            Some (fpub, Message.message
+              (Val.Vptr (stack_loc >> 2)) Vpubread bpub)).
+        { pose proof (Hpubread_new _ _ _ Hgetpub) as Hgetpub_new.
+          erewrite Cell.add_o in Hgetpub_new; eauto.
+          destruct (Time.eq_dec tpub tpubwrite);
+            [contradiction|done]. }
+        assert (Hpubmax : tpub = Cell.max_ts ζod).
+        { eapply cas_history_add_from_max; eauto. }
+        assert (Hofferd : offerd = Val.Vptr (stack_loc >> 2)).
+        { destruct CURod as (fcur & bcur & Hcur).
+          rewrite <- Hpubmax in Hcur. congruence. }
+        subst offerd.
+        assert (HVod : Vod = Vpubread).
+        { destruct CURod as (fcur & bcur & Hcur).
+          rewrite <- Hpubmax in Hcur. congruence. }
+        subst Vpubread.
+        change (View.le (TView.cur V11) Vpubwrite) in Hpubord.
+        rename Hpubord into Hcur11_pub.
+        assert (CURopub : current_message ζpubnew
+          (Val.Vptr offer_loc) Vpubwrite).
+        { eapply current_message_add; eauto. }
+        assert (CASHopub : cas_history ζpubnew).
+        { eapply cas_history_add; eauto. }
+        assert (PTRod' : pointer_history (stack_loc >> 2)
+          ((offer_loc, TView.cur V10) :: targetsd) ζod).
+        { eapply pointer_history_cons; exact PTRod. }
+        assert (PTRopub : pointer_history (stack_loc >> 2)
+          ((offer_loc, TView.cur V10) :: targetsd) ζpubnew).
+        { eapply pointer_history_add; [exact PTRod'| |exact HPUBADD].
+          exists (TView.cur V10). split; first (left; done).
+          right. etrans; [exact Hcur1011|exact Hcur11_pub]. }
+        assert (PTRhd' : pointer_history (stack_loc >> 2)
+          ((offer_loc, TView.cur V10) :: targetsd) ζhd).
+        { eapply pointer_history_cons; exact PTRhd. }
+        assert (LINKSd' : node_links (stack_loc >> 2)
+          ((offer_loc, TView.cur V10) :: targetsd) nodesd).
+        { eapply node_links_target_cons; exact LINKSd. }
+        destruct SENTd as (Vsentd & Hsentd).
+        iAssert (⌜current_message ζhd headd Vhd ∧ cas_history ζhd ∧
+          pointer_history (stack_loc >> 2)
+            ((offer_loc, TView.cur V10) :: targetsd) ζhd ∧
+          head_history (stack_loc >> 2) nodesd ζhd ∧
+          node_links (stack_loc >> 2)
+            ((offer_loc, TView.cur V10) :: targetsd) nodesd ∧
+          (∃ Vsent, (stack_loc >> 2, Vsent) ∈
+            ((offer_loc, TView.cur V10) :: targetsd))⌝)%I
+          as "#HPUREpub";
+          first (
+            iPureIntro;
+            split; [exact CURhd|];
+            split; [exact CASHhd|];
+            split; [exact PTRhd'|];
+            split; [exact HEADHd|];
+            split; [exact LINKSd'|];
+            exists Vsentd; right; exact Hsentd).
+        iAssert (⌜current_message ζpubnew (Val.Vptr offer_loc)
+            Vpubwrite ∧
+          cas_history ζpubnew ∧
+          pointer_history (stack_loc >> 2)
+            ((offer_loc, TView.cur V10) :: targetsd) ζpubnew⌝)%I
+          as "#OPUREpub"; first done.
+        assert (OFFER_NE : offer_loc ≠ stack_loc >> 2) by
+          (eapply base_loc_not_sentinel; eauto).
+        iMod (own_alloc (Excl ())) as "[%γoffer OfferTkn]"; first done.
+        iMod (hinv_alloc
+          (syn_offer_inv 0 γoffer offer_loc reqid value γs
+            (TView.cur V10) (TView.cur V10))
+          _ _ offerN with "[STATE OFFER2 HELP]")
+          as "[%γinv #Hoinv]"; eauto.
+        { solve_ndisj. }
+        { solve_base_sl_red.
+          iExists Val.zero,
+            (Cell.singleton (Message.message Val.zero Vos naos) LTos),
+            (Cell.singleton (Message.message Val.zero Vos naos) LTos),
+            (TView.cur V10), Vos, γstate.
+          iFrame "STATE SNstate".
+          iSplit.
+          { iPureIntro. repeat split.
+            - done.
+            - eexists fos, naos.
+              rewrite Cell.max_ts_singleton Cell.singleton_get. des_ifs.
+            - intros t f state Vstate b GET.
+              exists 0%Z. rewrite Cell.singleton_get in GET. des_ifs.
+            - intros t f state Vstate b GET.
+              left. rewrite Cell.max_ts_singleton.
+              rewrite Cell.singleton_get in GET. des_ifs.
+            - intros t f state Vstate b GET.
+              left. rewrite Cell.singleton_get in GET. des_ifs. }
+          simpl. iFrame "OFFER2 HELP". }
+        iAssert (is_offer 0 (stack_loc >> 2) γs
+          (Val.Vptr offer_loc) Vpubwrite)%I as "#OFFERpub".
+        { rewrite /is_offer.
+          destruct (decide (offer_loc = stack_loc >> 2)) as [HEQ|HNE].
+          - done.
+          - iExists (TView.cur V10), (TView.cur V10), γinv, γoffer,
+              value, reqid.
+            iSplit.
+            { iPureIntro. split.
+              - etrans; [exact Hcur1011|exact Hcur11_pub].
+              - etrans; [exact Hcur1011|exact Hcur11_pub]. }
+            iExact "Hoinv". }
+        iPoseProof (atomic_pts_to_seen_current
+          (stack_loc >> 1) γslot txod ζpubnew ζpubread CASOnly
+          (TView.cur V11) (Vbod ⊔ TView.cur V11)
+          (View.join_r _ _) with "SLOTd SNo11")
+          as "[SLOTd #SNopub]".
+        iMod ("ACC" with "[//]") as "[ACC _]".
+        iMod ("ACC" with
+          "[Hsd HEADd HPUREpub CHAINd SLOTd OPUREpub OFFERpub OFFER_TARGET TARGETSd REGd] IST")
+          as "IST".
+        { iEval (rewrite stack_inv'_eq; solve_base_sl_red).
+          iExists vsd, headd, (Val.Vptr offer_loc), ζhd, ζpubnew,
+            Vbhd, (Vbod ⊔ TView.cur V11), Vhd, Vpubwrite,
+            ((offer_loc, TView.cur V10) :: targetsd), nodesd.
+          solve_base_sl_red.
+          iFrame "Hsd HEADd HPUREpub CHAINd OPUREpub OFFERpub REGd".
+          iFrame "OFFER_TARGET TARGETSd".
+          rewrite syn_AtomicPtsTo_red AtomicPtsTo_eq /AtomicPtsTo_def.
+          iExists txod. iFrame. }
+        iEval (rewrite -IstHelp_nested_equiv) in "IST".
+        cStepsT. sYield. cStepsT. sYield. cStepsT.
+        iPoseProof (view_at_view_mon_pred
+          (view_at (AtomicSeen offer_loc γoffer_guard
+            (Cell.singleton (Message.message Val.zero Vog naog) LTog)))
+          _ _ Hcur1011 with "SNoffer10") as "#SNoffer11".
+        iEval (rewrite IstHelp_nested_equiv) in "IST".
+        iInv "Hinv" with "[IST]" as "[IST INVe]" "ACCe";
+          first by iFrame.
+        iEval (rewrite stack_inv'_eq; solve_base_sl_red) in "INVe".
+        iDestruct "INVe" as
+          (vse heade offere ζhe ζoe Vbhe Vboe Vhe Voe targetse nodese)
+          "[Hse [HEADe [HPUREe [CHAINe [SLOTe [OPUREe [OFFERe [TARGETSe REGe]]]]]]]]".
+        iEval (rewrite syn_AtomicPtsTo_red AtomicPtsTo_eq /AtomicPtsTo_def)
+          in "SLOTe".
+        iDestruct "SLOTe" as (txoe) "SLOTe".
+        iPoseProof (AtomicPtsToX_AtomicSeen_latest with "SLOTe SNopub")
+          as "%Hpub_cur".
+        destruct (Cell.add_get0 HPUBADD) as [_ Hgetpubwrite].
+        pose proof (Hpub_cur _ _ _ Hgetpubwrite) as Hgetpubwrite_e.
+        iPoseProof "HPUREe" as "#HPUREcopye".
+        iDestruct "HPUREcopye" as
+          %(CURhe & CASHhe & PTRhe & HEADHe & LINKSe & SENTe).
+        iPoseProof "OPUREe" as "#OPUREcopye".
+        iDestruct "OPUREcopye" as %(CURoe & CASHoe & PTRoe).
+        destruct (PTRoe _ _ _ _ _ Hgetpubwrite_e) as
+          (offer_e & Voguarde & EQoffer & Htargete & Hsafee).
+        inversion EQoffer; subst offer_e.
+        cInlineT.
+        cForceT (tid, stid, stack_loc >> 1, Val.Vptr offer_loc,
+          Val.Vptr (stack_loc >> 2), Ordering.relaxed, Ordering.acqrel,
+          V11, γslot, ζpubread, Vboe, txoe, ζoe, CASOnly,
+          target_pool targetse)%cris.
+        cForcesT.
+        iSplitL "TV SLOTe TARGETSe".
+        { iSplit.
+          { iPureIntro. reflexivity. }
+          iFrame "TV SNo11 SLOTe TARGETSe".
+          iSplit.
+          { iPureIntro. repeat split; eauto.
+            intros t f value0 V0 b Htime Hget0.
+            destruct (PTRoe _ _ _ _ _ Hget0) as
+              (loc0 & Vguard0 & EQ & IN & SAFE).
+            subst value0. done. }
+          iModIntro. iIntros "TARGETSe". iModIntro. iSplit.
+          { iDestruct (target_pool_lookup _ _ Htargete with "TARGETSe")
+              as "REC".
+            iDestruct (target_record_prim with "REC") as (q C Vp) "PRIM".
+            iExists q, C, Vp, γoffer_guard,
+              (Cell.singleton (Message.message Val.zero Vog naog) LTog).
+            iFrame "PRIM SNoffer11". }
+          iIntros (t f loc V0 b) "%OTHER".
+          destruct OTHER as (_ & GET & NE).
+          destruct (PTRoe _ _ _ _ _ GET) as
+            (loc2 & Vg2 & EQ & IN & SAFE). inversion EQ; subst loc2.
+          iDestruct (target_pool_lookup _ _ IN with "TARGETSe") as "REC".
+          iDestruct (target_record_prim with "REC") as (q C Vp) "PRIM".
+          iExists q, C, Vp. done. }
+        cStepT. cStepT. cStepT.
+        iDestruct "GRT" as
+          "[-> [%cleared [%ζclearread [%ζclearnew [%tclear [%fclear [%LTclear [%vclear [%Vclearread [%bclear [%V12 [HCLEAR [TV [#SNo12 [TARGETSe HCLEARCASE]]]]]]]]]]]]]]]".
+        iDestruct "HCLEAR" as
+          %[-> [Hseen1112 [Hclearread_new
+            [Hgetclear [Htimeclear HV1112]]]]].
+        iDestruct "HCLEARCASE" as "[CLEARFAIL|CLEARSUCC]".
+        { iDestruct "CLEARFAIL" as "[%CLEARFAIL SLOTe]".
+          destruct CLEARFAIL as (-> & Hclearneq & Hclearacq & ->).
+          iAssert (⌜current_message ζhe heade Vhe ∧ cas_history ζhe ∧
+            pointer_history (stack_loc >> 2) targetse ζhe ∧
+            head_history (stack_loc >> 2) nodese ζhe ∧
+            node_links (stack_loc >> 2) targetse nodese ∧
+            (∃ Vsent, (stack_loc >> 2, Vsent) ∈ targetse)⌝)%I
+            as "#HPUREe"; first done.
+          iAssert (⌜current_message ζclearnew offere Voe ∧
+            cas_history ζclearnew ∧
+            pointer_history (stack_loc >> 2) targetse ζclearnew⌝)%I
+            as "#OPUREe"; first done.
+          iMod ("ACCe" with "[//]") as "[ACCe _]".
+          iMod ("ACCe" with
+            "[Hse HEADe HPUREe CHAINe SLOTe OPUREe OFFERe TARGETSe REGe] IST")
+            as "IST".
+          { iEval (rewrite stack_inv'_eq; solve_base_sl_red).
+            iExists vse, heade, offere, ζhe, ζclearnew, Vbhe, Vboe,
+              Vhe, Voe, targetse, nodese.
+            solve_base_sl_red.
+            iFrame "Hse HEADe HPUREe CHAINe OPUREe OFFERe TARGETSe REGe".
+            rewrite syn_AtomicPtsTo_red AtomicPtsTo_eq /AtomicPtsTo_def.
+            iExists txoe. iFrame. }
+          iEval (rewrite -IstHelp_nested_equiv) in "IST".
+          shelve. }
+        { iDestruct "CLEARSUCC" as (Vclearwrite)
+            "[%CLEARSUCC [_ SLOTe]]".
+          destruct CLEARSUCC as
+            (-> & Heqclear & tclearwrite & HCLEARADD & Hclearvrw &
+              Hclearvrne & Hclearnotle & HclearneV & Hclearord).
+          subst vclear.
+          assert (Htclearwrite : Time.lt tclear tclearwrite) by
+            (eapply cell_add_lt; exact HCLEARADD).
+          assert (Htclear_ne : tclear ≠ tclearwrite) by
+            (intros ->; eapply Time.lt_strorder; exact Htclearwrite).
+          assert (Hgetclear_base :
+            Cell.get tclear ζoe =
+              Some (fclear, Message.message
+                (Val.Vptr offer_loc) Vclearread bclear)).
+          { pose proof (Hclearread_new _ _ _ Hgetclear) as Hgetclear_new.
+            erewrite Cell.add_o in Hgetclear_new; eauto.
+            destruct (Time.eq_dec tclear tclearwrite);
+              [contradiction|done]. }
+          assert (Hclearmax : tclear = Cell.max_ts ζoe).
+          { eapply cas_history_add_from_max; eauto. }
+          assert (Hoffere : offere = Val.Vptr offer_loc).
+          { destruct CURoe as (fcur & bcur & Hcur).
+            rewrite <- Hclearmax in Hcur. congruence. }
+          subst offere.
+          assert (HVoe : Voe = Vclearread).
+          { destruct CURoe as (fcur & bcur & Hcur).
+            rewrite <- Hclearmax in Hcur. congruence. }
+          subst Vclearread.
+          change (View.le (TView.cur V12) Vclearwrite) in Hclearord.
+          rename Hclearord into Hcur12_clear.
+          assert (CURoclear : current_message ζclearnew
+            (Val.Vptr (stack_loc >> 2)) Vclearwrite).
+          { eapply current_message_add; eauto. }
+          assert (CASHoclear : cas_history ζclearnew).
+          { eapply cas_history_add; eauto. }
+          destruct SENTe as (Vsente & Hsente).
+          assert (PTRoclear : pointer_history (stack_loc >> 2)
+            targetse ζclearnew).
+          { eapply pointer_history_add; [exact PTRoe| |exact HCLEARADD].
+            exists Vsente. split; first exact Hsente. left; done. }
+          iAssert (⌜current_message ζhe heade Vhe ∧ cas_history ζhe ∧
+            pointer_history (stack_loc >> 2) targetse ζhe ∧
+            head_history (stack_loc >> 2) nodese ζhe ∧
+            node_links (stack_loc >> 2) targetse nodese ∧
+            (∃ Vsent, (stack_loc >> 2, Vsent) ∈ targetse)⌝)%I
+            as "#HPUREe".
+          { iPureIntro.
+            split; [exact CURhe|].
+            split; [exact CASHhe|].
+            split; [exact PTRhe|].
+            split; [exact HEADHe|].
+            split; [exact LINKSe|].
+            exists Vsente. exact Hsente. }
+          iAssert (⌜current_message ζclearnew
+              (Val.Vptr (stack_loc >> 2)) Vclearwrite ∧
+            cas_history ζclearnew ∧
+            pointer_history (stack_loc >> 2) targetse ζclearnew⌝)%I
+            as "#OPUREclear"; first done.
+          iAssert (is_offer 0 (stack_loc >> 2) γs
+            (Val.Vptr (stack_loc >> 2)) Vclearwrite)%I
+            as "#OFFERclear".
+          { rewrite /is_offer.
+            destruct (decide (stack_loc >> 2 = stack_loc >> 2))
+              as [HEQ|HNE].
+            - done.
+            - exfalso. apply HNE. reflexivity. }
+          iMod ("ACCe" with "[//]") as "[ACCe _]".
+          iMod ("ACCe" with
+            "[Hse HEADe HPUREe CHAINe SLOTe OPUREclear OFFERclear TARGETSe REGe] IST")
+            as "IST".
+          { iEval (rewrite stack_inv'_eq; solve_base_sl_red).
+            iExists vse, heade, (Val.Vptr (stack_loc >> 2)), ζhe,
+              ζclearnew, Vbhe, (Vboe ⊔ TView.cur V12), Vhe,
+              Vclearwrite, targetse, nodese.
+            solve_base_sl_red.
+            iFrame "Hse HEADe HPUREe CHAINe OPUREclear OFFERclear TARGETSe REGe".
+            rewrite syn_AtomicPtsTo_red AtomicPtsTo_eq /AtomicPtsTo_def.
+            iExists txoe. iFrame. }
+          iEval (rewrite -IstHelp_nested_equiv) in "IST".
+          shelve. }
+        Unshelve.
+        all: sYield; cStepsT; sYield; cStepsT;
+          iEval (rewrite IstHelp_nested_equiv) in "IST";
+          iInv "Hoinv" with "[IST]" as "[IST OINV]" "OACC".
+        all: try (by iFrame).
+        all: iEval (solve_base_sl_red) in "OINV";
+          iDestruct "OINV" as
+            (state ζstate ζstate_seen Vbstate Vmsgstate γstate')
+            "[STATE [#SNstate' [STATEPURE OSTATE]]]";
+          iDestruct "STATEPURE" as
+            %(Hstate_seen & CURstate & NUMstate & CASHstate & STATEHIST);
+          inversion HV1112 as [Hrel1112 Hcur1112 Hacq1112];
+          assert (Hcur1012 : View.le (TView.cur V10) (TView.cur V12)) by
+            (etrans; [exact Hcur1011|exact Hcur1112]);
+          iPoseProof (view_at_view_mon_pred
+            (view_at (AtomicSeen (offer_loc >> 1) γstate' ζstate_seen))
+            _ _ Hcur1012 with "SNstate'") as "#SNstate12";
+          iEval (rewrite AtomicPtsTo_eq /AtomicPtsTo_def) in "STATE";
+          iDestruct "STATE" as (txstate) "STATE";
+          cInlineT;
+          cForceT (tid, stid, offer_loc >> 1, Val.zero, Val.Vnum 2,
+            Ordering.acqrel, Ordering.acqrel, V12, γstate', ζstate_seen,
+            Vbstate, txstate, ζstate, CASOnly, emp%I)%cris;
+          cForcesT;
+          iSplitL "TV STATE".
+        all: try (
+          iSplit;
+          [ iPureIntro; repeat split; eauto
+          | iFrame "TV SNstate12 STATE";
+            iSplit;
+            [ iPureIntro; repeat split; eauto;
+              intros t f v V0 b _ Hget0;
+              destruct (NUMstate _ _ _ _ _ Hget0) as [z ->]; done
+            | solve_base_sl_red ] ]).
+        all: cStepsT;
+          iDestruct "GRT" as
+            "[-> [%withdrew [%ζstate_read [%ζstate_new [%tstate [%fstate [%LTstate [%vstate [%Vstate_read [%bstate [%V13 [HWITHDRAW [TV [#SNstate13 [_ HWITHDRAWCASE]]]]]]]]]]]]]]]";
+          iDestruct "HWITHDRAW" as
+            %[-> [Hstate_seen1213 [Hstate_read_new
+              [Hstate_get [Htstate HV1213]]]]];
+          iDestruct "HWITHDRAWCASE" as "[WITHDRAWFAIL|WITHDRAWSUCC]".
+        2: shelve.
+        3: shelve.
+        all: (
+          iDestruct "WITHDRAWFAIL" as "[%WITHDRAWFAIL STATE]";
+          destruct WITHDRAWFAIL as
+            (-> & Hwithdrawneq & Hwithdrawacq & ->);
+          pose proof (Hstate_read_new _ _ _ Hstate_get)
+            as Hstate_get_full;
+          destruct (STATEHIST _ _ _ _ _ Hstate_get_full)
+            as [Hstate_zero|Hstate_current];
+          [ subst vstate; contradiction
+          | subst vstate;
+            destruct (NUMstate _ _ _ _ _ Hstate_get_full)
+              as (z & Hstate_num);
+            subst state;
+            iEval (simpl) in "OSTATE";
+            destruct_decide (decide (z = 0%Z)) as Hz0;
+            [ subst z; contradiction
+            | destruct_decide (decide (z = 1%Z)) as Hz1;
+              [ subst z;
+                iPoseProof "OSTATE" as "#Done";
+                iAssert (@{Vbstate} (offer_loc >> 1) cas↦{γstate'}
+                  ζstate_new)%I with "[STATE]" as "STATE";
+                [ rewrite AtomicPtsTo_eq /AtomicPtsTo_def;
+                  iExists txstate; done
+                |];
+                iMod ("OACC" with "[//]") as "[OACC _]";
+                iMod ("OACC" with "[STATE Done] IST") as "IST";
+                [ solve_base_sl_red;
+                  iExists Val.one, ζstate_new, ζstate_seen,
+                    Vbstate, Vmsgstate, γstate';
+                  iFrame "STATE SNstate' Done"; done
+                |];
+                iEval (rewrite -IstHelp_nested_equiv) in "IST";
+                cStepsT; sYield; cStepsT;
+                sYieldS;
+                iApply (wsim_HelpDone_try_run with "Done");
+                cStepsS; sYieldS; cStepsS; cForcesS;
+                iSplitL "TV";
+                [ iSplit;
+                  [ done
+                  | iExists V13; iSplit; [done|iFrame "TV"] ]
+                |];
+                cStepsS; cStepsT; cStep; iFrame "IST"; done
+              | destruct_decide (decide (z = 2%Z)) as Hz2;
+                [ subst z; iCombine "OfferTkn OSTATE" gives %WF; done
+                | done ]
+              ]
+            ]
+          ]).
+        Unshelve.
+        all: (
+          iDestruct "WITHDRAWSUCC" as (Vstate_write)
+            "[%WITHDRAWSUCC [_ STATE]]";
+          destruct WITHDRAWSUCC as
+            (-> & Heqwithdraw & tstate_write & HSTATEADD & Hstatevrw &
+              Hstatevrne & Hstatenotle & HstateneV & Hstateord);
+          subst vstate;
+          assert (Htstate_write : Time.lt tstate tstate_write) by
+            (eapply cell_add_lt; exact HSTATEADD);
+          assert (Htstate_ne : tstate ≠ tstate_write) by
+            (intros ->; eapply Time.lt_strorder; exact Htstate_write);
+          assert (Hstate_get_base :
+            Cell.get tstate ζstate =
+              Some (fstate,
+                Message.message Val.zero Vstate_read bstate)) by
+            (pose proof (Hstate_read_new _ _ _ Hstate_get) as Hget_new;
+             erewrite Cell.add_o in Hget_new; eauto;
+             destruct (Time.eq_dec tstate tstate_write);
+               [contradiction|done]);
+          assert (Hstatemax : tstate = Cell.max_ts ζstate) by
+            (eapply cas_history_add_from_max; eauto);
+          assert (Hstatezero : state = Val.zero) by
+            (destruct CURstate as (fcur & bcur & Hcur);
+             rewrite <- Hstatemax in Hcur; congruence);
+          subst state;
+          iEval (simpl) in "OSTATE";
+          iDestruct "OSTATE" as "[PAYLOAD HELP]";
+          change (Vstate_write = TView.cur V13) in Hstateord;
+          subst Vstate_write;
+          assert (CURstate_new : current_message ζstate_new
+            (Val.Vnum 2) (TView.cur V13)) by
+            (eapply current_message_add; eauto);
+          assert (NUMstate_new : numeric_history ζstate_new) by
+            (eapply numeric_history_add; eauto);
+          assert (CASHstate_new : cas_history ζstate_new) by
+            (eapply cas_history_add; eauto);
+          assert (STATEHISTnew :
+            offer_state_history ζstate_new (Val.Vnum 2)) by
+            (eapply offer_state_history_add_from_zero; eauto);
+          assert (Hstate_seen_new : Cell.le ζstate_seen ζstate_new) by
+            (etrans; eauto);
+          iAssert (@{Vbstate ⊔ TView.cur V13}
+            (offer_loc >> 1) cas↦{γstate'} ζstate_new)%I
+            with "[STATE]" as "STATE";
+          [ rewrite AtomicPtsTo_eq /AtomicPtsTo_def;
+            iExists txstate; done
+          |];
+          iMod ("OACC" with "[//]") as "[OACC _]";
+          iMod ("OACC" with "[STATE OfferTkn] IST") as "IST";
+          [ solve_base_sl_red;
+            iExists (Val.Vnum 2), ζstate_new, ζstate_seen,
+              (Vbstate ⊔ TView.cur V13), (TView.cur V13), γstate';
+            iFrame "STATE SNstate'";
+            iSplit;
+            [ done
+            | simpl; repeat case_decide; try lia; iFrame "OfferTkn" ]
+          |];
+          iEval (rewrite -IstHelp_nested_equiv) in "IST";
+          cStepsT; sYield; cStepsT;
+          inversion HV1213 as [Hrel1213 Hcur1213 Hacq1213];
+          assert (HcurV13 : View.le (TView.cur V) (TView.cur V13)) by
+            (etrans; [exact HcurV10|]; etrans; [exact Hcur1011|];
+              etrans; [exact Hcur1112|exact Hcur1213]);
+          iPoseProof (view_at_view_mon_pred
+            (view_at (AtomicSeen stack_loc γh ζh_seen)) _ _ HcurV13
+            with "SNh") as "#SNh13";
+          iPoseProof (view_at_view_mon_pred
+            (view_at (AtomicSeen (stack_loc >> 1) γslot ζclearread))
+            _ _ Hcur1213 with "SNo12") as "#SNo13";
+          iPoseProof (view_at_view_mon_pred
+            (view_at (AtomicSeen (stack_loc >> 2) γguard ζguard))
+            _ _ HcurV13 with "SNg") as "#SNg13";
+          iAssert (stack_handle γs (Val.Vptr stack_loc) (TView.cur V13))%I
+            with "[]" as "#HANDLE13";
+          [ rewrite /stack_handle;
+            iExists stack_loc, γstackinv, γh, γslot, ζh_seen, ζclearread,
+              γguard, ζguard, γnm;
+            iSplit; [done|iFrame "Hinv SNh13 SNo13 SNg13"]
+          |];
+          unfold CS__, cris_s;
+          rewrite (push_postcond_irrel value γs tid stid V V13);
+          cNormS;
+          unfold CT__, cris_t; cNormT;
+          cByCoind CIH; iFrame "HANDLE13 TV IST HELP WINV").
+      }
+    - iDestruct "SUCCESS" as (Vw) "[%SUCC [_ HEADc]]".
+      clear CIH.
+      destruct SUCC as
+        (-> & Heq & twrite & HADD & Hvrw & Hvrne &
+          Hnotle & HneqV & Hord).
+      subst vseen.
+      assert (Htwrite : Time.lt tcas twrite) by
+        (eapply cell_add_lt; exact HADD).
+      assert (Htcas_ne : tcas ≠ twrite) by
+        (intros ->; eapply Time.lt_strorder; exact Htwrite).
+      assert (Hget_base :
+        Cell.get tcas ζhc =
+          Some (fcas, Message.message (Val.Vptr head_loc) Vread bcas)).
+      { pose proof (Hafter_new _ _ _ Hgetcas) as Hget_new.
+        erewrite Cell.add_o in Hget_new; eauto.
+        destruct (Time.eq_dec tcas twrite); [contradiction|done]. }
+      assert (Hmax : tcas = Cell.max_ts ζhc).
+      { eapply cas_history_add_from_max; eauto. }
+      pose proof CURhc as CURhc0.
+      assert (Hheadc : headc = Val.Vptr head_loc).
+      { destruct CURhc0 as (fcur & bcur & Hcur).
+        rewrite <- Hmax in Hcur. congruence. }
+      subst headc.
+      inversion HV56 as [Hrel56 Hcur56 Hacq56].
+      change (View.le (TView.cur V6) Vw) in Hord.
+      assert (Hpubw : View.le (TView.cur V5) Vw) by
+        (etrans; [exact Hcur56|exact Hord]).
+      assert (Hmsg5 : View.le Vmsg (TView.cur V5)) by
+        (etrans; [exact HVmsg|exact Hcur15]).
+      assert (NEWLINK :
+        dnew.(node_next) = stack_loc >> 2 ∨
+          ∃ dnext Vnext,
+            nodesc !! dnew.(node_next) = Some dnext ∧
+            (dnew.(node_next), Vnext) ∈ targetsc ∧
+            View.le dnext.(node_pub_view) dnew.(node_pub_view) ∧
+            View.le Vnext dnew.(node_pub_view)).
+      { rewrite /dnew /=.
+        destruct (decide (head_loc = stack_loc >> 2))
+          as [->|Hnext_ne]; first by left.
+        right.
+        destruct (head_history_lookup _ _ _ _ _ _ _ _
+          Hnext_ne Hget_cur HEADHc) as (dnext & LOOKnext & LEpubnext).
+        destruct Hsafec as [HSENT|LEguard]; first contradiction.
+        exists dnext, Vguardc.
+        split; [exact LOOKnext|].
+        split; [exact Htargetc|].
+        split.
+        - etrans; [exact LEpubnext|exact Hmsg5].
+        - etrans; [exact LEguard|exact Hmsg5]. }
+      assert (CURhnew : current_message ζnew (Val.Vptr node) Vw).
+      { eapply current_message_add; eauto. }
+      assert (CASHhnew : cas_history ζnew).
+      { eapply cas_history_add; eauto. }
+      assert (PTRhc' : pointer_history (stack_loc >> 2)
+        ((node, TView.cur V5) :: targetsc) ζhc).
+      { eapply pointer_history_cons; exact PTRhc. }
+      assert (PTRhnew : pointer_history (stack_loc >> 2)
+        ((node, TView.cur V5) :: targetsc) ζnew).
+      { eapply pointer_history_add; [exact PTRhc'| |exact HADD].
+        exists (TView.cur V5). split; first (left; done).
+        right. exact Hpubw. }
+      assert (HEADHc' : head_history (stack_loc >> 2)
+        (<[node := dnew]> nodesc) ζhc).
+      { eapply head_history_insert; eauto. }
+      assert (HEADHnew : head_history (stack_loc >> 2)
+        (<[node := dnew]> nodesc) ζnew).
+      { eapply head_history_add; [exact HEADHc'| |exact HADD].
+        right. exists dnew. split; first by rewrite lookup_insert.
+        rewrite /dnew /=. exact Hpubw. }
+      assert (LINKSnew : node_links (stack_loc >> 2)
+        ((node, TView.cur V5) :: targetsc)
+        (<[node := dnew]> nodesc)).
+      { eapply (node_links_insert (stack_loc >> 2) targetsc nodesc
+          node dnew (TView.cur V5)); eauto. }
+      iDestruct "OPUREc" as %(CURoc & CASHoc & PTRoc).
+      assert (PTRoc' : pointer_history (stack_loc >> 2)
+        ((node, TView.cur V5) :: targetsc) ζoc).
+      { eapply pointer_history_cons; exact PTRoc. }
+      destruct SENTc as (Vsentc & Hsentc).
+      iAssert (⌜current_message ζnew (Val.Vptr node) Vw ∧
+        cas_history ζnew ∧
+        pointer_history (stack_loc >> 2)
+          ((node, TView.cur V5) :: targetsc) ζnew ∧
+        head_history (stack_loc >> 2)
+          (<[node := dnew]> nodesc) ζnew ∧
+        node_links (stack_loc >> 2)
+          ((node, TView.cur V5) :: targetsc)
+          (<[node := dnew]> nodesc) ∧
+        (∃ Vsent, (stack_loc >> 2, Vsent) ∈
+          ((node, TView.cur V5) :: targetsc))⌝)%I
+        as "#HPUREnew".
+      { iPureIntro.
+        split; [exact CURhnew|].
+        split; [exact CASHhnew|].
+        split; [exact PTRhnew|].
+        split; [exact HEADHnew|].
+        split; [exact LINKSnew|].
+        exists Vsentc. right. exact Hsentc. }
+      iAssert (⌜current_message ζoc offerc Voc ∧
+        cas_history ζoc ∧
+        pointer_history (stack_loc >> 2)
+          ((node, TView.cur V5) :: targetsc) ζoc⌝)%I
+        as "#OPUREnew"; first done.
+      iPoseProof (live_chain_insert_mono
+        (stack_loc >> 2) nodesc vsc (Val.Vptr head_loc) node dnew FRESH
+        with "CHAINc") as "CHAINoldnew".
+      iAssert (live_chain (stack_loc >> 2)
+        (<[node := dnew]> nodesc) (value :: vsc) (Val.Vptr node))%I
+        with "[NEW_VALUE CHAINoldnew]" as "CHAINnew".
+      { simpl. iExists node, dnew. rewrite /dnew /=.
+        iSplit.
+        { iPureIntro. repeat split; eauto. by rewrite lookup_insert. }
+        iFrame. }
+      iMod (node_registry_insert γnm nodesc node dnew FRESH
+        with "NEW_NODE REGc") as "REGc".
+      iMod ("ACC" with "[//]") as "[_ > ACC]".
+      sYieldS. prependRetT tt.
+      iApply (wsim_helping_pend_try_run with "HELP [-]").
+      aUnfoldS. rewrite /StackM.jobCode.
+      cNormS. sYieldS. cStepsS.
+      iDestruct (stack_content_auth_agree with "Hsc ASM") as %Hstack.
+      subst _q.
+      subst _q0.
+      iMod (stack_content_auth_update γs vsc (value :: vsc)
+        with "Hsc ASM") as "[Hsc ASM]".
+      cForcesS; first iFrame "ASM".
+      cStep.
+      iFrame "WINV".
+      iIntros "#Done".
+      cStepsS.
+      iMod ("ACC" with
+        "[Hsc HEADc HPUREnew CHAINnew SLOTc OPUREnew OFFERc NEW_TARGET TARGETSc REGc] IST")
+        as "IST".
+      { iEval (rewrite stack_inv'_eq; solve_base_sl_red).
+        iExists (value :: vsc), (Val.Vptr node), offerc,
+          ζnew, ζoc, (Vbhc ⊔ TView.cur V6), Vboc, Vw, Voc,
+          ((node, TView.cur V5) :: targetsc), (<[node := dnew]> nodesc).
+        solve_base_sl_red.
+        iFrame "Hsc HPUREnew CHAINnew SLOTc OPUREnew OFFERc REGc".
+        iFrame "NEW_TARGET TARGETSc".
+        rewrite syn_AtomicPtsTo_red AtomicPtsTo_eq /AtomicPtsTo_def.
+        iExists txhc. iFrame. }
+      iEval (rewrite -IstHelp_nested_equiv) in "IST".
+      cStepsT. sYield. cStepsT.
+      sYieldS. cStepsS. cForcesS.
+      iSplitL "TV".
+      { iSplit; first done.
+        iExists V6. iSplit; first done. iFrame "TV". }
+      cStepsS. cStepsT. cStep. iFrame "IST". done.
+  Qed.
+End StackIM.
