concurrent/promise_free/system/SystemIACAS.v
@@ -1,0 +1,87 @@
+Require Import CRIS.common.CRIS.
+From CRIS.promise_free.system Require Import SystemHeader SystemI SystemA.
+From CRIS.promise_free.pfmem Require Import PFMemHeader PFMemA.
+From CRIS.promise_free.algebra Require Import HistoryRA AtomicRA.
+
+Section SystemIA.
+  Import SystemA.
+  Context `{!crisG Γ Σ α β τ _S _I, _HIST: !histGS, _ATOMIC: !atomicG, _SYS: !sysGS}.
+  Context (sp_user sp : specmap).
+  Context (size : list Z).
+  Context (Hincl : sp_user ⊆ sp).
+  Context (Hsysincl : (SystemA.sp sp_user ⊤) ⊆ sp).
+
+  Local Definition SystemA_s := SystemA.t sp_user ⊤ sp ★ PFMemA.t sp.
+  Local Definition SystemI_s := SystemI.t ★ PFMemA.t sp.
+
+  Definition Ist : ist_type Σ :=
+    λ st_src st_tgt,
+      (∃ (tid : Ident.t) (tids : gmap Ident.t (TView.t * nat)),
+        let tids' : gmap Ident.t nat := snd <$> tids in
+        ⌜st_tgt = {[SystemI.v_tid # tid↑; SystemI.v_tids # tids'↑]} ∧
+         st_src = {[SystemI.v_tid # tid↑; SystemI.v_tids # tids'↑]}⌝ ∗
+        tview_sys_auth tids ∗
+        ([∗ map] i ↦ stid ∈ (snd <$> delete tid tids), YIELD stid))%I.
+
+  Local Definition IstFull :=
+    (IstProd (IstSB (Mod.scopes (SystemA.t sp_user ⊤ sp)) Ist) IstEq).
+
+  Lemma simF_cas : ISim.sim_fun open SystemA_s SystemI_s IstFull (fid SystemHdr.cas).
+  Proof using.
+    cStartFunSim. rewrite /SystemI.cas. cStepsS.
+    destruct _q as [[[[[[[[[[[[[[tid stid] loc] old] new] ordr] ordw] V]
+      γ] ζ'] Vb] tx] ζ] mode] Pr].
+    iDestruct "ASM" as "[-> [PURE [TV [SN [PT [AW [PR CMP]]]]]]]".
+    iDestruct "PURE" as "[-> %PRE]".
+    iDestruct "TV" as "[Tid STV]".
+    iDestruct "IST" as (????) "[[-> ->] [[% IST] ->]]".
+    iDestruct "IST" as "[%tid_cur [%tids [[-> ->] [TA YS]]]]".
+
+    iPoseProof (tview_sys_lookup with "TA Tid") as "%Hlookup"; first iFrame.
+    destruct (decide (tid = tid_cur)); cycle 1.
+    { iPoseProof (big_sepM_lookup_acc with "YS") as "[TV2 YS]".
+      { instantiate (2:=tid). rewrite lookup_fmap lookup_delete_ne // Hlookup; ss. }
+      iDestruct "STV" as "[_ Y2]".
+      iPoseProof (YieldToken_both with "Y2 TV2") as "%"; done.
+    }
+    subst.
+
+    cStepsT. rewrite /SystemI.get_tid. cStepsT. cInlineT.
+    cForceT (tid_cur, loc, old, new, ordr, ordw, V, γ, ζ', Vb, tx, ζ, mode, Pr)%cris.
+    iDestruct "TA" as "[TA TVS]".
+    cForcesT. iFrame.
+    rewrite big_sepM_delete //=. iDestruct "TVS" as "[$ TVS]"; eauto.
+    iSplit; eauto.
+    cStepsT.
+    iDestruct "GRT" as
+      "[-> [%ret [%ζ'' [%ζn [%t' [%f' [%LT [%v' [%Vr [%b [%V' [PURE [TV [SN [PR RESULT]]]]]]]]]]]]]]]".
+    iDestruct "PURE" as "[-> %POST]".
+
+    iCombine "TA" "Tid" as "TA".
+    iMod (own_update with "TA") as "TA".
+    { rewrite (gmap_view_replace _ tid_cur _ (to_agree _)) //. }
+    iDestruct "TA" as "[TA Tid]".
+
+    cForcesS.
+    iSplitL "Tid STV SN PR RESULT".
+    { iSplitR; first eauto.
+      iExists ret, ζ'', ζn, t', f', LT, v', Vr, b, V'.
+      iSplitR; first (iPureIntro; eauto).
+      iFrame.
+    }
+    cStepsT.
+    cStep.
+
+    iSplit; eauto.
+    iExists _, _, _, _; iSplit; eauto.
+    iSplit; eauto.
+    iSplit; eauto.
+    iExists tid_cur, (<[tid_cur := (V', stid)]> tids); iSplit.
+    { iPureIntro; split; rewrite fmap_insert /=; f_equal;
+        rewrite insert_id // lookup_fmap Hlookup //.
+    }
+    rewrite -fmap_insert /=; iFrame. rewrite delete_insert_delete.
+    iSplitL "TVS TV"; eauto.
+    rewrite big_sepM_insert_delete; iFrame.
+  Qed.
+End SystemIA.
